forall in zk

generic/GenericZeroKnowledge.ec
@@ -59,6 +59,635 @@ module ZKIdeal(S: Simulator, V: RewMaliciousVerifier, D: ZKDistinguisher) = {
 
 
 
+
+abstract theory SequentialCompositionZK.
+
+(* op s : statement. *)
+(* op w : witness. *)
+op n : int.
+
+(* axiom zkrel_prop : zk_relation s w. *)
+
+module ZKRealAmp(P: HonestProver, V: MaliciousVerifier, D: ZKDistinguisher) = {
+  proc run(statement: statement, witness: witness) = {
+    var commit, challenge, response, summary, guess,i;
+     i <- 0;
+     summary <- Pervasive.witness;
+     while(i < n){
+       commit <@ P.commitment(statement, witness);
+       challenge <@ V.challenge(statement, commit);
+       response <@ P.response(challenge);
+       summary <@ V.summitup(statement, response);
+       i <- i + 1;
+     }
+    guess <@ D.guess(statement, witness, summary);
+    return guess;
+  }
+}.
+
+
+module SimAmp(S: Simulator, V : RewMaliciousVerifier) = { 
+  proc simulate(statement:statement) = { 
+   var summary, i; 
+   i <- 0;
+   summary <- witness;
+   while(i < n) { 
+     summary <@ S(V).simulate(statement); 
+     i <- i + 1;
+   } 
+   return summary; 
+  } 
+}.
+
+
+require HybridWithArg2.
+(* q -> N *)
+clone import HybridWithArg2 as Hyb with type input <- unit,
+                                type output <- adv_summary,
+                                type outputA <- bool,
+                                type argt <- statement * witness,
+                                op q <- n.
+
+
+module Ad(D : ZKDistinguisher, Ob : Orclb, O : Orcl) = {
+  proc main(s:statement,w:witness) : bool = {
+    var summary, guess,i;
+    i <- 0;
+    summary <- witness;
+    while (i < n){
+       summary <@ O.orcl((s,w));
+       i <- i + 1;
+    }
+    guess <@ D.guess(s, w, summary);
+    return guess;
+  }
+}.
+
+
+module Obb(P : HonestProver, V : RewMaliciousVerifier, Sim : Simulator) = {
+  proc leaks(x:inleaks) : outleaks = {
+    return witness;
+  }
+  proc orclR(s:statement, w: witness) : adv_summary = {
+    var commit, challenge, response, summary;
+    commit <@ P.commitment(s, w);
+    challenge <@ V.challenge(s, commit);
+    response <@ P.response(challenge);
+    summary <@ V.summitup(s, response);
+    return summary;
+  }
+  proc orclL(s:statement, w: witness) : adv_summary = {
+    var summary;
+    summary <@ Sim(V).simulate(s);
+    return summary;
+  }
+}.
+
+require  MemoryPropsLE.
+clone import MemoryPropsLE with type at2 <- statement * witness,
+                                        type at1 <- statement * witness.
+
+
+section.
+
+
+declare module Q <: HonestProver.
+declare module P <: HonestProver{-Q, -HybOrcl, -Count}.
+declare module Sim <: Simulator{-Q, -HybOrcl, -P, -Count}.
+declare module V <: RewMaliciousVerifier {-Q, -HybOrcl, -P, -Sim, -Count}.
+declare module D <: ZKDistinguisher{-Q, - Count}. 
+
+
+declare axiom sim_run_ll : forall (V0 <: RewMaliciousVerifier),  
+     islossless V0.challenge => islossless V0.summitup => islossless Sim(V0).simulate.
+declare axiom V_summitup_ll  : islossless V.summitup.
+declare axiom V_challenge_ll : islossless V.challenge.
+declare axiom P_response_ll : islossless P.response.
+declare axiom P_commitment_ll : islossless P.commitment.
+declare axiom D_guess_ll     : islossless D.guess.
+
+declare axiom q_ge1 : 1 <= n. 
+
+declare axiom D_guess_prop : equiv[ D.guess ~ D.guess : ={glob V, arg} ==> ={res} ].
+
+module Ob = Obb(P,V,Sim).
+module A = Ad(D).
+
+
+
+module Y = {
+  proc main(s:statement, w: witness) = {
+   var summary, guess;
+   HybOrcl.l0 <$ [0..max 0 (n-1)];
+   HybOrcl.l <- 0;
+   summary <- witness;
+   while (HybOrcl.l < n && HybOrcl.l < HybOrcl.l0) {
+     summary <@
+       HybOrcl(Ob, R(Ob)).orcl(s,w);
+   }
+   while (HybOrcl.l < n && HybOrcl.l0 <= HybOrcl.l) {
+     summary <@
+       HybOrcl(Ob, R(Ob)).orcl(s,w);
+   }
+   guess <@ D.guess(s, w, summary);
+   return guess;
+ }
+}.
+module Z = {
+  proc main(s:statement, w:witness) = {
+   var summary, guess;
+   HybOrcl.l0 <$ [0..max 0 (n -1 )];
+   HybOrcl.l <- 0;
+   summary <- witness;
+   while (HybOrcl.l < n && HybOrcl.l < HybOrcl.l0) {
+     summary <@
+       HybOrcl(Ob, L(Ob)).orcl(s,w);
+   }
+   while (HybOrcl.l < n && HybOrcl.l0 <= HybOrcl.l) {
+     summary <@
+       HybOrcl(Ob, L(Ob)).orcl(s,w);
+   }
+   guess <@ D.guess(s, w, summary);
+   return guess;
+ }
+}.
+module Z2 = {
+  proc main(s:statement, w:witness) = {
+   var summary, guess;
+   HybOrcl.l0 <$ [0..max 0 (n -1 )];
+   HybOrcl.l <- 0;
+   summary <- witness;
+   while (HybOrcl.l < n && HybOrcl.l < HybOrcl.l0) {
+     summary <@
+       HybOrcl(Ob, L(Ob)).orcl(s,w);
+   }
+   if(HybOrcl.l < n && HybOrcl.l0 <= HybOrcl.l){
+     summary <@
+       HybOrcl(Ob, L(Ob)).orcl(s,w);
+   }
+   while (HybOrcl.l < n && HybOrcl.l0 <= HybOrcl.l) {
+     summary <@
+       HybOrcl(Ob, L(Ob)).orcl(s,w);
+   }
+   guess <@ D.guess(s, w, summary);
+   return guess;
+ }
+}.
+module Y2 = {
+  proc main(s:statement, w:witness) = {
+   var summary, guess;
+   HybOrcl.l0 <$ [0..max 0 (n -1 )];
+   HybOrcl.l <- 0;
+   summary <- witness;
+   while (HybOrcl.l < n && HybOrcl.l < HybOrcl.l0) {
+     summary <@
+       HybOrcl(Ob, R(Ob)).orcl(s,w);
+   }
+   if(HybOrcl.l < n && HybOrcl.l0 <= HybOrcl.l){
+     summary <@
+       HybOrcl(Ob, R(Ob)).orcl(s,w);
+   }
+   while (HybOrcl.l < n && HybOrcl.l0 <= HybOrcl.l) {
+     summary <@
+       HybOrcl(Ob, R(Ob)).orcl(s,w);
+   }
+   guess <@ D.guess(s, w, summary);
+   return guess;
+ }
+}.
+module Z3 = {
+  proc main(s:statement, w:witness) = {
+    var commit, challenge, response, summary, guess;
+   HybOrcl.l0 <$ [0..max 0 (n -1 )];
+   HybOrcl.l <- 0;
+   summary <- witness;
+   while (HybOrcl.l < n && HybOrcl.l < HybOrcl.l0) {
+     commit <@ P.commitment(s, w);
+     challenge <@ V.challenge(s, commit);
+     response <@ P.response(challenge);
+     summary <@ V.summitup(s, response);
+     HybOrcl.l <- HybOrcl.l + 1;
+   }
+   summary <@ Sim(V).simulate(s);
+   HybOrcl.l <- HybOrcl.l + 1;
+   while (HybOrcl.l < n) {
+    summary <@ Sim(V).simulate(s);
+    HybOrcl.l <- HybOrcl.l + 1;
+   }
+   guess <@ D.guess(s, w, summary);
+   return guess;
+ }
+}.
+module Y3 = {
+  proc main(s:statement, w:witness) = {
+    var commit, challenge, response, summary, guess;
+   HybOrcl.l0 <$ [0..max 0 (n -1 )];
+   HybOrcl.l <- 0;
+   summary <- witness;
+   while (HybOrcl.l < n && HybOrcl.l < HybOrcl.l0) {
+     commit <@ P.commitment(s, w);
+     challenge <@ V.challenge(s, commit);
+     response <@ P.response(challenge);
+     summary <@ V.summitup(s, response);
+     HybOrcl.l <- HybOrcl.l + 1;
+   }
+     commit <@ P.commitment(s, w);
+     challenge <@ V.challenge(s, commit);
+     response <@ P.response(challenge);
+     summary <@ V.summitup(s, response);
+   HybOrcl.l <- HybOrcl.l + 1;
+   while (HybOrcl.l < n) {
+    summary <@ Sim(V).simulate(s);
+    HybOrcl.l <- HybOrcl.l + 1;
+   }
+   guess <@ D.guess(s, w, summary);
+   return guess;
+ }
+}.
+local lemma y &m ss ww:
+  Pr[Y2.main(ss,ww) @ &m : res] = Pr[Y3.main(ss,ww) @ &m : res].
+byequiv(_: ={glob D, glob V, glob P, glob Sim, glob HybOrcl, arg} ==> _).
+proc.
+seq 6 10 : (={summary, glob V,s,w}).
+seq 4 4 : (={s,w,HybOrcl.l, HybOrcl.l0, glob V, glob P, glob Sim, summary} /\ HybOrcl.l0{2} = HybOrcl.l{2} /\ HybOrcl.l0{2} < n 
+ /\ HybOrcl.l{2} < n
+   ).
+while (={s,w,glob V, glob P, HybOrcl.l, HybOrcl.l0, glob V, glob P, glob Sim, summary} /\ HybOrcl.l{2} <= HybOrcl.l0{2}  /\ HybOrcl.l0{2} < n  ). inline*.
+sp.
+rcondf {1} 1 . progress. skip. smt.
+rcondf {1} 1 . progress. skip. smt.    
+sp. wp. call (_:true).
+call (_:true). call (_:true).
+call (_:true). skip. progress. smt. 
+wp. rnd. skip. progress.  smt. smt. smt. smt.
+rcondt {1} 1. progress. 
+seq 1 5 : (={s,w,HybOrcl.l, HybOrcl.l0, glob V, glob P, glob Sim, summary} /\
+  HybOrcl.l0{2} < HybOrcl.l{2} /\ HybOrcl.l0{2} < n  /\ HybOrcl.l{2} <= n ).
+inline HybOrcl(Ob, R(Ob)).orcl. sp. 
+rcondf {1} 1. progress. 
+rcondt {1} 1. progress. 
+inline*.
+sp. wp.  
+call (_:true). call (_:true).
+call (_:true). call (_:true). skip. progress. smt.  smt.
+while (={s,w,HybOrcl.l, HybOrcl.l0, glob V, glob P, glob Sim, summary} /\
+  HybOrcl.l0{2} < HybOrcl.l{2} /\ HybOrcl.l0{2} < n).
+inline*. sp.
+rcondt {1} 1. progress. 
+sp.  wp.  call (_: ={glob V}). sim. sim. sim. sim. skip. progress. smt. 
+smt.    skip. progress. smt.
+call D_guess_prop. skip.  
+auto. auto. auto.
+qed.
+local lemma w ss ww &m :
+  Pr[Z2.main(ss,ww) @ &m : res] =
+    Pr[Z3.main(ss,ww) @ &m : res].
+byequiv(_: ={s,w,glob D, glob V, glob P, glob Sim, glob HybOrcl} ==> _).
+proc.
+seq 6 7 : (={s,w,summary, glob V}).
+seq 4 4 : (={s,w,HybOrcl.l, HybOrcl.l0, glob V, glob P, glob Sim, summary} /\ HybOrcl.l0{2} = HybOrcl.l{2} /\ HybOrcl.l0{2} < n 
+ /\ HybOrcl.l{2} <= n
+   ).
+while (={s,w,glob V, glob P, HybOrcl.l, HybOrcl.l0, glob V, glob P, glob Sim, summary} /\ HybOrcl.l{2} <= HybOrcl.l0{2}  /\ HybOrcl.l0{2} < n  ). inline*.
+sp.
+rcondf {1} 1 . progress. skip. smt.
+rcondf {1} 1 . progress. skip. smt.    
+sp. wp. call (_:true).
+call (_:true). call (_:true).
+call (_:true). skip. progress. smt. 
+wp. rnd. skip. progress.  smt. smt. smt. smt.
+rcondt {1} 1. progress.  
+seq 1 2 : (={HybOrcl.l, HybOrcl.l0, glob V, glob P, glob Sim, summary,s,w} /\
+  HybOrcl.l0{2} < HybOrcl.l{2} /\ HybOrcl.l0{2} < n  /\ HybOrcl.l{2} <= n).
+inline HybOrcl(Ob, L(Ob)).orcl. sp. 
+rcondf {1} 1. progress. 
+rcondt {1} 1. progress. 
+inline*.
+sp. wp.  
+call (_: ={glob V}). sim. sim. sim. sim. skip. progress. smt. smt.
+while (={HybOrcl.l, HybOrcl.l0, glob V, glob P, glob Sim, summary, s, w} /\
+  HybOrcl.l0{2} < HybOrcl.l{2} /\ HybOrcl.l0{2} < n).
+inline*. sp.
+rcondt {1} 1. progress. 
+sp.  wp.  call (_: ={glob V}). sim. sim. sim. sim. skip. progress. smt. 
+smt.   skip. progress. smt.
+call D_guess_prop. auto.
+auto. auto.
+qed.
+
+local lemma yy ss ww &m : 
+  Pr[Y.main(ss,ww) @ &m : res] = 
+    Pr[Y2.main(ss,ww) @ &m : res].
+byequiv(_: ={s,w,glob D, glob V, glob P, glob Sim, glob HybOrcl} ==> _).
+proc. 
+unroll {1} 5.
+seq 6 6 : (={s,w,summary, glob V}).
+sim. call D_guess_prop. skip. auto.
+auto. auto.
+qed.
+local lemma ww ss ww' &m : 
+  Pr[Z.main(ss,ww') @ &m : res] = 
+    Pr[Z2.main(ss,ww') @ &m : res].
+byequiv(_: ={s,w,glob D, glob V, glob P, glob Sim, glob HybOrcl} ==> _).
+proc. 
+unroll {1} 5.
+seq 6 6 : (={s,w,summary, glob V}).
+sim.
+call D_guess_prop. skip. auto.
+auto. auto.
+qed.
+
+lemma www ss ww &m : 
+  Pr[HybGame(A,Ob,L(Ob)).main(ss,ww) @ &m : res] = 
+  Pr[Z.main(ss,ww) @ &m : res].
+byequiv(_: ma{1} = (s,w){2} /\ ={glob D, glob V, glob P, glob Sim} ==> _).
+proc.
+inline {1} A(Ob, HybOrcl(Ob, L(Ob))).main.
+splitwhile {1} 6 : (i < HybOrcl.l0).
+seq 6 4 : (={s,w,glob V, glob P, HybOrcl.l, HybOrcl.l0, glob V, glob P, glob Sim, summary} /\
+  i{1} = HybOrcl.l{2} /\ HybOrcl.l0{2} <= HybOrcl.l{2}).
+simplify. wp.
+while (={s,w,glob V, glob P, HybOrcl.l, HybOrcl.l0, glob V, glob P, glob Sim, summary} /\
+  i{1} = HybOrcl.l{2}). inline*.
+sp.
+rcondf {1} 1 . progress. skip.   progress.  smt.
+rcondf {2} 1 . progress. skip.   progress.  smt.
+rcondf {1} 1 . progress. skip.   progress.  smt.
+rcondf {2} 1 . progress. skip.   progress.  smt.
+sp. wp.  call (_:true). call (_:true). call (_:true). call (_:true).
+skip. progress.
+wp. rnd. skip. progress. smt.
+wp. 
+seq 1 1 : (={s,w,summary, glob V}).
+while (={s,w,glob V, glob P, HybOrcl.l, HybOrcl.l0, glob V, glob P, glob Sim, summary} /\
+  i{1} = HybOrcl.l{2} /\ HybOrcl.l0{2} <= HybOrcl.l{2} ). 
+wp. simplify. 
+inline HybOrcl(Ob, L(Ob)).orcl.
+wp. sp. if. progress. inline*. wp. 
+call (_: ={glob V}). sim. sim. sim. sim. 
+wp. skip. progress. smt. smt. 
+rcondt {1} 1. progress. skip. progress. smt.
+rcondt {2} 1. progress. skip. progress. smt.
+inline*. wp.
+call (_: ={glob V}). sim. sim. sim. sim. 
+wp.  skip. progress. smt. smt.  
+skip. progress.  
+call D_guess_prop. skip. auto.
+auto.
+auto.
+qed.
+lemma yyy ss ww &m : 
+  Pr[HybGame(A,Ob,R(Ob)).main(ss,ww) @ &m : res] = 
+  Pr[Y.main(ss,ww) @ &m : res].
+byequiv(_: ={arg,glob D, glob V, glob P, glob Sim} ==> _).
+proc.
+inline {1} A(Ob, HybOrcl(Ob, R(Ob))).main.
+splitwhile {1} 6 : (i < HybOrcl.l0).
+seq 6 4 : (={s,w,glob V, glob P, HybOrcl.l, HybOrcl.l0, glob V, glob P, glob Sim, summary} /\
+  i{1} = HybOrcl.l{2} /\ HybOrcl.l0{2} <= HybOrcl.l{2}).
+simplify.
+while (={s,w,glob V, glob P, HybOrcl.l, HybOrcl.l0, glob V, glob P, glob Sim, summary} /\
+  i{1} = HybOrcl.l{2}). inline*.
+sp.
+rcondf {1} 1 . progress. skip.   progress.  smt.
+rcondf {2} 1 . progress. skip.   progress.  smt.
+rcondf {1} 1 . progress. skip.   progress.  smt.
+rcondf {2} 1 . progress. skip.   progress.  smt.
+sp. wp.  call (_:true). call (_:true). call (_:true). call (_:true).
+skip. progress.
+wp. rnd. skip. progress. smt.
+wp. 
+seq 1 1 : (={s,w,summary, glob V, glob HybOrcl}).
+while (={s,w,glob V, glob P, HybOrcl.l, HybOrcl.l0, glob V, glob P, glob Sim, summary} /\
+  i{1} = HybOrcl.l{2} /\ HybOrcl.l0{2} <= HybOrcl.l{2} ). 
+wp. simplify. 
+inline HybOrcl(Ob, R(Ob)).orcl.
+wp. sp. if. progress. inline*. wp. 
+call (_: ={glob V, glob HybOrcl}). sim. sim. sim. sim. 
+wp. skip. progress. smt. smt. 
+rcondt {1} 1. progress. skip. progress. smt.
+rcondt {2} 1. progress. skip. progress. smt.
+inline*. wp. sp.  call (_:true). call (_:true). call (_:true). call (_:true).
+skip. progress. smt. smt.
+skip. progress.  call D_guess_prop. skip. auto.
+auto.
+auto.
+qed.
+
+lemma qq ss ww &m:
+        Pr[Ln(Ob,A).main(ss,ww) @ &m : res]
+      - Pr[Rn(Ob,A).main(ss,ww) @ &m : res]
+    = n%r *(Pr[HybGame(A,Ob,L(Ob)).main(ss,ww) @ &m : res]
+            - Pr[HybGame(A,Ob,R(Ob)).main(ss,ww) @ &m : res]).
+apply (Hybrid_restr Ob A _ _ _ _ _ &m (fun _ _ _ r => r)).
+progress. proc. inline*.
+wp.  call (_:true). 
+while (Count.c = i /\ i <= n) . wp. 
+call (_:true). wp.  skip.  progress. smt.
+wp.  skip.  progress. smt.
+proc. skip. auto. proc.
+call (sim_run_ll V). apply V_challenge_ll.
+apply V_summitup_ll. skip. auto.
+proc. call V_summitup_ll. call P_response_ll.
+call V_challenge_ll. call P_commitment_ll. skip. auto.
+progress.
+proc. call D_guess_ll. sp.
+while (true) (n - i + 1). progress.
+wp. call H. skip. progress. smt.
+progress. skip. progress. smt.
+qed.
+
+
+
+module Ob1 = Obb(P,V,Sim).
+module A1 = Ad(D).
+
+module Amem : IR1R2 = {
+  proc init(s:statement, w:witness) = {
+   var commit, challenge, response, summary;
+   HybOrcl.l0 <$ [0..max 0 (n -1 )];
+   HybOrcl.l <- 0;
+   summary <- witness;
+   while (HybOrcl.l < n && HybOrcl.l < HybOrcl.l0) {
+     commit <@ P.commitment(s, w);
+     challenge <@ V.challenge(s, commit);
+     response <@ P.response(challenge);
+     summary <@ V.summitup(s, response);
+     HybOrcl.l <- HybOrcl.l + 1;
+   }
+  }
+  proc run1(s:statement, w:witness) = {
+   var  summary, guess;
+   summary <@ Sim(V).simulate(s);
+   HybOrcl.l <- HybOrcl.l + 1;
+   while (HybOrcl.l < n) {
+    summary <@ Sim(V).simulate(s);
+    HybOrcl.l <- HybOrcl.l + 1;
+   }
+   guess <@ D.guess(s, w, summary);
+   return guess;
+  }
+  proc run2(s:statement, w:witness) = {
+   var commit, challenge, response, summary, guess;
+   commit <@ P.commitment(s, w);
+   challenge <@ V.challenge(s, commit);
+   response <@ P.response(challenge);
+   summary <@ V.summitup(s, response);
+   HybOrcl.l <- HybOrcl.l + 1;
+   while (HybOrcl.l < n) {
+    summary <@ Sim(V).simulate(s);
+    HybOrcl.l <- HybOrcl.l + 1;
+   }
+   guess <@ D.guess(s, w, summary);
+   return guess;
+  }
+}.
+
+module Dstar : ZKDistinguisher = {
+  proc guess(s : statement, w: witness, summary: adv_summary) = {
+   var guess;
+   HybOrcl.l <- HybOrcl.l + 1;
+   while (HybOrcl.l < n) {
+    summary <@ Sim(V).simulate(s);
+    HybOrcl.l <- HybOrcl.l + 1;
+   }
+   guess <@ D.guess(s, w,  summary);
+   return guess;
+  }
+}.
+
+
+local lemma lll (ss : statement) (ww : witness) &m deltoid : 
+   (forall &n,
+   Pr[ZKIdeal(Sim, V, Dstar).run(ss, ww) @ &n : res]
+    - Pr[ZKReal(P, V, Dstar).run(ss, ww) @ &n : res] 
+           < deltoid) =>
+   Pr[HybGame(A1,Ob1,L(Ob1)).main(ss,ww) @ &m : res]
+               - Pr[HybGame(A1,Ob1,R(Ob1)).main(ss,ww) @ &m : res] < deltoid.
+move => zk_ass.
+have ->: Pr[HybGame(A1,Ob1,L(Ob1)).main(ss,ww) @ &m : res] =
+         Pr[MemoryPropsLE.P(Amem).main1((ss,ww),(ss,ww)) @ &m : res].
+rewrite www. rewrite ww. rewrite w.
+byequiv. proc. 
+inline Amem.run1. inline Amem.init.
+wp.  seq 7 9 : (={glob V} /\ (s,w){1} = (s,w){2} /\ summary{1} = summary{2} ).  sp. wp. 
+seq 4 4 : (={glob HybOrcl, glob V, glob P} /\ (s,w){1} = (s0,w0){2} /\ summary{1} = summary0{2} /\ (s,w){1} = i2{2}).
+while (={glob V, glob P, glob HybOrcl} /\ (s,w){1} = (s0,w0){2}
+ /\ summary{1} = summary0{2} /\ (s,w){1} = i2{2}).
+wp.  call (_:true). call (_:true). call (_:true).  call (_:true).
+skip. progress. wp.  rnd. skip. progress. smt. smt. 
+sp.
+seq 2 2 : (={glob P, glob V,  glob HybOrcl, summary, s, w}).
+wp.  call (_: ={glob V}). sim. sim. sim. sim.
+skip. progress.         
+while (={glob V, glob P, glob HybOrcl} /\ (s,w){1} = (s,w){2}
+ /\ summary{1} = summary{2}) . wp. 
+call (_: ={glob V}).  sim. sim. sim. sim.
+skip. progress. 
+skip. progress. 
+call D_guess_prop. skip. auto.
+auto. auto. 
+
+
+have ->: Pr[HybGame(A1,Ob1,R(Ob1)).main(ss,ww) @ &m : res] =
+         Pr[MemoryPropsLE.P(Amem).main2((ss,ww),(ss,ww)) @ &m : res].
+rewrite yyy. rewrite yy. rewrite y.
+byequiv. proc. 
+inline Amem.run2. inline Amem.init.
+wp. seq 10 12 : (={s,w,summary, glob V}). 
+sim. wp.
+
+while (={glob V, glob P, glob HybOrcl} /\ (s,w){1} = (s0,w0){2}
+ /\ summary{1} = summary0{2} /\ (s,w){1} = i2{2}).
+
+wp.  call (_:true). call (_:true). call (_:true).  call (_:true).
+skip. progress. wp.  rnd. wp. skip. progress. smt. smt. 
+
+
+
+call D_guess_prop. skip. auto.
+auto. auto.
+case (Pr[MemoryPropsLE.P(Amem).main1((ss,ww), (ss,ww)) @ &m : res] -
+Pr[MemoryPropsLE.P(Amem).main2((ss,ww),(ss,ww)) @ &m : res] < deltoid). auto.
+move => q.
+have zz : Pr[MemoryPropsLE.P(Amem).main1((ss,ww),(ss,ww)) @ &m : res] -
+  Pr[MemoryPropsLE.P(Amem).main2((ss,ww),(ss,ww)) @ &m : res] >= deltoid. 
+smt. clear q.
+have ko : exists &n, deltoid <= Pr[Amem.run1((ss,ww)) @ &n : res] - Pr[Amem.run2((ss,ww)) @ &n : res].
+apply (o_o Amem (ss, ww) (ss, ww) &m).  auto.
+elim ko. move => &n. move => q.
+have ok : Pr[Amem.run1((ss, ww)) @ &n : res] - Pr[Amem.run2((ss, ww)) @ &n : res] < deltoid.
+
+
+have -> : Pr[Amem.run1((ss, ww)) @ &n : res] = Pr[ZKIdeal(Sim, V, Dstar).run(ss, ww) @ &n : res].
+byequiv. proc.         
+inline Dstar.guess. wp.
+seq 3 6: (={glob V,s,w} /\ summary{1} = summary0{2} /\  HybOrcl.l{1} =  HybOrcl.l{2}). sim. 
+progress. smt. smt.
+call D_guess_prop. skip. auto.
+auto.  auto. 
+
+have -> : Pr[Amem.run2((ss, ww)) @ &n : res] = Pr[ZKReal(P, V, Dstar).run(ss, ww) @ &n : res].
+byequiv. proc.         
+inline Dstar.guess. wp.
+seq 6 9: (={glob V,s,w} /\ summary{1} = summary0{2} /\ HybOrcl.l{1} = HybOrcl.l{2}). sim. 
+
+progress. smt. smt. smt.
+call D_guess_prop. skip. progress.
+auto.  auto. 
+apply (zk_ass  &n ). smt. 
+qed.
+
+
+
+lemma zk_seq &m deltoid ss ww : 
+   (forall &n,
+   Pr[ZKIdeal(Sim, V, Dstar).run(ss, ww) @ &n : res]
+    - Pr[ZKReal(P, V, Dstar).run(ss, ww) @ &n : res] 
+           < deltoid) =>
+   Pr[ZKIdeal(SimAmp(Sim), V, D).run(ss, ww) @ &m : res]
+        - Pr[ZKRealAmp(P, V, D).run(ss, ww) @ &m : res]
+          < n%r * deltoid.
+move => zk_ass.
+have -> : Pr[ZKIdeal(SimAmp(Sim), V, D).run(ss, ww) @ &m : res]
+ = Pr[Ln(Ob,A).main(ss,ww) @ &m : res].
+byequiv (_:   
+  (glob V){2} = (glob V){m} /\ ={glob Sim, arg}/\
+  (statement{1}, witness{1}, n{1}) = (ss, ww, n) /\
+   (glob V){1} = (glob V){m} ==> _). 
+
+proc. inline*. wp. sp.
+seq 2 1 : (={glob V, summary} /\ statement{1} = s{2} /\ witness{1} = w{2}).   wp.
+while (={i, glob V, glob Sim} /\ summary0{1} = summary{2} /\ statement0{1} = s{2} /\ witness{1} = w{2} ).
+wp. call (_: ={glob V}). sim. sim. sim. sim. wp.  skip. progress.
+skip. progress.
+
+
+call D_guess_prop. skip. auto. auto. auto.
+have -> : Pr[ZKRealAmp(P, V, D).run(ss, ww) @ &m : res]
+ = Pr[Rn(Ob,A).main(ss,ww) @ &m : res].
+byequiv (_: ={glob V, glob P, arg} /\ (statement{1}, witness{1}) = (ss, ww) ==> _). proc.
+inline*. wp. sp.
+seq 1 1 : (={glob V, summary} /\ statement{1} = s{2} /\ witness{1} = w{2} ).   simplify. wp.
+while (={i, glob V, glob P} /\ summary{1} = summary{2} /\ statement{1} = s{2} /\  witness{1} = w{2}). sp. wp.
+call (_:true). call (_:true). call (_:true). call (_:true). skip. progress. 
+
+
+
+skip. progress. call D_guess_prop. skip.  auto. auto. auto.
+rewrite qq.
+have :  Pr[HybGame(A1,Ob1,L(Ob1)).main(ss,ww) @ &m : res]
+               - Pr[HybGame(A1,Ob1,R(Ob1)).main(ss,ww) @ &m : res] < deltoid.
+apply lll. smt. smt.
+qed.
+
+
+end section.
+
+end SequentialCompositionZK.
+
+
+
 abstract theory OneShotSimulator.
 
 op zk_error : statement -> int -> real.
@@ -130,14 +759,13 @@ module  Simulator(S : Simulator1)(V : RewMaliciousVerifier)  = {
 
    declare axiom D_guess_prop : equiv[ D.guess ~ D.guess : ={glob V, arg} ==> ={res} ].
 
-    lemma computational_statisticalVpoly_zk stat wit p0 negl &m:
+    lemma computational_zk stat wit p0 negl &m:
        zk_relation stat wit =>
        `|Pr[W0(Sim1(V), D).run(stat, wit) @ &m : fst res.`2 /\ res.`1] /
             Pr[Sim1(V).run(stat) @ &m : fst res]
         - Pr[ ZKD(HonestProver,V,D).main(stat,wit) @ &m : res ]| <= negl =>
 
        p0 <= Pr[Sim1(V).run(stat) @ &m : res.`1] =>
-
        let real_prob = Pr[ZKReal(HonestProver, V, D).run(stat, wit) @ &m : res] in
        let ideal_prob = Pr[ZKIdeal(Simulator(Sim1), V, D).run(stat, wit) @ &m : res] in
          `|real_prob - ideal_prob| <= negl + 2%r * (1%r - p0)^n.
@@ -261,595 +889,19 @@ module  Simulator(S : Simulator1)(V : RewMaliciousVerifier)  = {
   apply (sim1_run_ll V).  apply V_challenge_ll. apply V_summitup_ll. apply sim1_rew_ph. apply D_guess_ll. auto.
    apply (qqq &m stat wit  D V);auto.  apply D_guess_ll. apply V_summitup_ll. apply V_challenge_ll. apply V_rew. apply n_pos. smt.  auto.
    qed.
+
+
+
+   (* clone import SequentialCompositionZK as SCZK. *)
+
+   (* lemma statistical_zk_seq stat wit p0 &m: *)
+   (*     zk_relation stat wit =>  *)
+   (*     p0 <= Pr[Sim1(V).run(stat) @ &m : res.`1] => *)
+   (*     let real_prob = Pr[ZKRealSeq(HonestProver, V, D).run(stat, wit) @ &m : res] in *)
+   (*     let ideal_prob = Pr[ZKIdeal(SimulatorAmp(Simulator(Sim1)), V, D).run(stat, wit) @ &m : res] in *)
+   (*       `|real_prob - ideal_prob| <= negl + 2%r * (1%r - p0)^n. *)
+
   end section.
   end StatisticalZK.
 end OneShotSimulator.
-
-
-
-abstract theory SequentialCompositionZK.
-
-op s : statement.
-op w : witness.
-op n : int.
-
-axiom zkrel_prop : zk_relation s w.
-
-module ZKRealAmp(P: HonestProver, V: MaliciousVerifier, D: ZKDistinguisher) = {
-  proc run(statement: statement, witness: witness) = {
-    var commit, challenge, response, summary, guess,i;
-     i <- 0;
-     summary <- Pervasive.witness;
-     while(i < n){
-       commit <@ P.commitment(statement, witness);
-       challenge <@ V.challenge(statement, commit);
-       response <@ P.response(challenge);
-       summary <@ V.summitup(statement, response);
-       i <- i + 1;
-     }
-    guess <@ D.guess(statement, witness, summary);
-    return guess;
-  }
-}.
-
-
-module SimAmp(S: Simulator, V : RewMaliciousVerifier) = { 
-  proc simulate(statement:statement) = { 
-   var summary, i; 
-   i <- 0;
-   summary <- witness;
-   while(i < n) { 
-     summary <@ S(V).simulate(statement); 
-     i <- i + 1;
-   } 
-   return summary; 
-  } 
-}.
-
-
-require Hybrid.
-(* q -> N *)
-clone import Hybrid as Hyb with type input <- unit,
-                                type output <- adv_summary,
-                                type outputA <- bool,
-                                op q <- n.
-
-
-module Ad(D : ZKDistinguisher, Ob : Orclb, O : Orcl) = {
-  proc main() : bool = {
-    var summary, guess,i;
-    i <- 0;
-    summary <- witness;
-    while (i < n){
-       summary <@ O.orcl();
-       i <- i + 1;
-    }
-    guess <@ D.guess(s, w, summary);
-    return guess;
-  }
-}.
-
-
-module Obb(P : HonestProver, V : RewMaliciousVerifier, Sim : Simulator) = {
-  proc leaks(x:inleaks) : outleaks = {
-    return witness;
-  }
-  proc orclR() : adv_summary = {
-    var commit, challenge, response, summary;
-    commit <@ P.commitment(s, w);
-    challenge <@ V.challenge(s, commit);
-    response <@ P.response(challenge);
-    summary <@ V.summitup(s, response);
-    return summary;
-  }
-  proc orclL() : adv_summary = {
-    var summary;
-    summary <@ Sim(V).simulate(s);
-    return summary;
-  }
-}.
-
-require import MemoryPropsLE.
-
-
-section.
-
-
-declare module Q <: HonestProver.
-declare module P <: HonestProver{-Q, -HybOrcl, -Count}.
-declare module Sim <: Simulator{-Q, -HybOrcl, -P, -Count}.
-declare module V <: RewMaliciousVerifier {-Q, -HybOrcl, -P, -Sim, -Count}.
-declare module D <: ZKDistinguisher{-Q, - Count}. 
-
-
-declare axiom sim_run_ll : forall (V0 <: RewMaliciousVerifier),  
-     islossless V0.challenge => islossless V0.summitup => islossless Sim(V0).simulate.
-declare axiom V_summitup_ll  : islossless V.summitup.
-declare axiom V_challenge_ll : islossless V.challenge.
-declare axiom P_response_ll : islossless P.response.
-declare axiom P_commitment_ll : islossless P.commitment.
-declare axiom D_guess_ll     : islossless D.guess.
-
-declare axiom q_ge1 : 1 <= n. 
-
-declare axiom D_guess_prop : equiv[ D.guess ~ D.guess : ={glob V, arg} ==> ={res} ].
-
-module Ob = Obb(P,V,Sim).
-module A = Ad(D).
-
-
-
-module Y = {
-  proc main() = {
-   var summary, guess;
-   HybOrcl.l0 <$ [0..max 0 (n-1)];
-   HybOrcl.l <- 0;
-   summary <- witness;
-   while (HybOrcl.l < n && HybOrcl.l < HybOrcl.l0) {
-     summary <@
-       HybOrcl(Ob, R(Ob)).orcl();
-   }
-   while (HybOrcl.l < n && HybOrcl.l0 <= HybOrcl.l) {
-     summary <@
-       HybOrcl(Ob, R(Ob)).orcl();
-   }
-   guess <@ D.guess(s, w, summary);
-   return guess;
- }
-}.
-module Z = {
-  proc main() = {
-   var summary, guess;
-   HybOrcl.l0 <$ [0..max 0 (n -1 )];
-   HybOrcl.l <- 0;
-   summary <- witness;
-   while (HybOrcl.l < n && HybOrcl.l < HybOrcl.l0) {
-     summary <@
-       HybOrcl(Ob, L(Ob)).orcl();
-   }
-   while (HybOrcl.l < n && HybOrcl.l0 <= HybOrcl.l) {
-     summary <@
-       HybOrcl(Ob, L(Ob)).orcl();
-   }
-   guess <@ D.guess(s, w, summary);
-   return guess;
- }
-}.
-module Z2 = {
-  proc main() = {
-   var summary, guess;
-   HybOrcl.l0 <$ [0..max 0 (n -1 )];
-   HybOrcl.l <- 0;
-   summary <- witness;
-   while (HybOrcl.l < n && HybOrcl.l < HybOrcl.l0) {
-     summary <@
-       HybOrcl(Ob, L(Ob)).orcl();
-   }
-   if(HybOrcl.l < n && HybOrcl.l0 <= HybOrcl.l){
-     summary <@
-       HybOrcl(Ob, L(Ob)).orcl();
-   }
-   while (HybOrcl.l < n && HybOrcl.l0 <= HybOrcl.l) {
-     summary <@
-       HybOrcl(Ob, L(Ob)).orcl();
-   }
-   guess <@ D.guess(s, w, summary);
-   return guess;
- }
-}.
-module Y2 = {
-  proc main() = {
-   var summary, guess;
-   HybOrcl.l0 <$ [0..max 0 (n -1 )];
-   HybOrcl.l <- 0;
-   summary <- witness;
-   while (HybOrcl.l < n && HybOrcl.l < HybOrcl.l0) {
-     summary <@
-       HybOrcl(Ob, R(Ob)).orcl();
-   }
-   if(HybOrcl.l < n && HybOrcl.l0 <= HybOrcl.l){
-     summary <@
-       HybOrcl(Ob, R(Ob)).orcl();
-   }
-   while (HybOrcl.l < n && HybOrcl.l0 <= HybOrcl.l) {
-     summary <@
-       HybOrcl(Ob, R(Ob)).orcl();
-   }
-   guess <@ D.guess(s, w, summary);
-   return guess;
- }
-}.
-module Z3 = {
-  proc main() = {
-    var commit, challenge, response, summary, guess;
-   HybOrcl.l0 <$ [0..max 0 (n -1 )];
-   HybOrcl.l <- 0;
-   summary <- witness;
-   while (HybOrcl.l < n && HybOrcl.l < HybOrcl.l0) {
-     commit <@ P.commitment(s, w);
-     challenge <@ V.challenge(s, commit);
-     response <@ P.response(challenge);
-     summary <@ V.summitup(s, response);
-     HybOrcl.l <- HybOrcl.l + 1;
-   }
-   summary <@ Sim(V).simulate(s);
-   HybOrcl.l <- HybOrcl.l + 1;
-   while (HybOrcl.l < n) {
-    summary <@ Sim(V).simulate(s);
-    HybOrcl.l <- HybOrcl.l + 1;
-   }
-   guess <@ D.guess(s, w, summary);
-   return guess;
- }
-}.
-module Y3 = {
-  proc main() = {
-    var commit, challenge, response, summary, guess;
-   HybOrcl.l0 <$ [0..max 0 (n -1 )];
-   HybOrcl.l <- 0;
-   summary <- witness;
-   while (HybOrcl.l < n && HybOrcl.l < HybOrcl.l0) {
-     commit <@ P.commitment(s, w);
-     challenge <@ V.challenge(s, commit);
-     response <@ P.response(challenge);
-     summary <@ V.summitup(s, response);
-     HybOrcl.l <- HybOrcl.l + 1;
-   }
-     commit <@ P.commitment(s, w);
-     challenge <@ V.challenge(s, commit);
-     response <@ P.response(challenge);
-     summary <@ V.summitup(s, response);
-   HybOrcl.l <- HybOrcl.l + 1;
-   while (HybOrcl.l < n) {
-    summary <@ Sim(V).simulate(s);
-    HybOrcl.l <- HybOrcl.l + 1;
-   }
-   guess <@ D.guess(s, w, summary);
-   return guess;
- }
-}.
-local lemma y &m :
-  Pr[Y2.main() @ &m : res] = Pr[Y3.main() @ &m : res].
-byequiv(_: ={glob D, glob V, glob P, glob Sim, glob HybOrcl} ==> _).
-proc.
-seq 6 10 : (={summary, glob V}).
-seq 4 4 : (={HybOrcl.l, HybOrcl.l0, glob V, glob P, glob Sim, summary} /\ HybOrcl.l0{2} = HybOrcl.l{2} /\ HybOrcl.l0{2} < n 
- /\ HybOrcl.l{2} < n
-   ).
-while (={glob V, glob P, HybOrcl.l, HybOrcl.l0, glob V, glob P, glob Sim, summary} /\ HybOrcl.l{2} <= HybOrcl.l0{2}  /\ HybOrcl.l0{2} < n  ). inline*.
-sp.
-rcondf {1} 1 . progress. skip. smt.
-rcondf {1} 1 . progress. skip. smt.    
-sp. wp. call (_:true).
-call (_:true). call (_:true).
-call (_:true). skip. progress. smt. 
-wp. rnd. skip. progress.  smt. smt. smt. smt.
-rcondt {1} 1. progress. 
-seq 1 5 : (={HybOrcl.l, HybOrcl.l0, glob V, glob P, glob Sim, summary} /\
-  HybOrcl.l0{2} < HybOrcl.l{2} /\ HybOrcl.l0{2} < n  /\ HybOrcl.l{2} <= n ).
-inline HybOrcl(Ob, R(Ob)).orcl. sp. 
-rcondf {1} 1. progress. 
-rcondt {1} 1. progress. 
-inline*.
-sp. wp.  
-call (_:true). call (_:true).
-call (_:true). call (_:true). skip. progress. smt.  smt.
-while (={HybOrcl.l, HybOrcl.l0, glob V, glob P, glob Sim, summary} /\
-  HybOrcl.l0{2} < HybOrcl.l{2} /\ HybOrcl.l0{2} < n).
-inline*. sp.
-rcondt {1} 1. progress. 
-sp.  wp.  call (_: ={glob V}). sim. sim. sim. sim. skip. progress. smt. 
-smt.    skip. progress. smt.
-call D_guess_prop. skip.  
-auto. auto. auto.
-qed.
-local lemma w &m :
-  Pr[Z2.main() @ &m : res] =
-    Pr[Z3.main() @ &m : res].
-byequiv(_: ={glob D, glob V, glob P, glob Sim, glob HybOrcl} ==> _).
-proc.
-seq 6 7 : (={summary, glob V}).
-seq 4 4 : (={HybOrcl.l, HybOrcl.l0, glob V, glob P, glob Sim, summary} /\ HybOrcl.l0{2} = HybOrcl.l{2} /\ HybOrcl.l0{2} < n 
- /\ HybOrcl.l{2} <= n
-   ).
-while (={glob V, glob P, HybOrcl.l, HybOrcl.l0, glob V, glob P, glob Sim, summary} /\ HybOrcl.l{2} <= HybOrcl.l0{2}  /\ HybOrcl.l0{2} < n  ). inline*.
-sp.
-rcondf {1} 1 . progress. skip. smt.
-rcondf {1} 1 . progress. skip. smt.    
-sp. wp. call (_:true).
-call (_:true). call (_:true).
-call (_:true). skip. progress. smt. 
-wp. rnd. skip. progress.  smt. smt. smt. smt.
-rcondt {1} 1. progress.  
-seq 1 2 : (={HybOrcl.l, HybOrcl.l0, glob V, glob P, glob Sim, summary} /\
-  HybOrcl.l0{2} < HybOrcl.l{2} /\ HybOrcl.l0{2} < n  /\ HybOrcl.l{2} <= n).
-inline HybOrcl(Ob, L(Ob)).orcl. sp. 
-rcondf {1} 1. progress. 
-rcondt {1} 1. progress. 
-inline*.
-sp. wp.  
-call (_: ={glob V}). sim. sim. sim. sim. skip. progress. smt. smt.
-while (={HybOrcl.l, HybOrcl.l0, glob V, glob P, glob Sim, summary} /\
-  HybOrcl.l0{2} < HybOrcl.l{2} /\ HybOrcl.l0{2} < n).
-inline*. sp.
-rcondt {1} 1. progress. 
-sp.  wp.  call (_: ={glob V}). sim. sim. sim. sim. skip. progress. smt. 
-smt.   skip. progress. smt.
-call D_guess_prop. auto.
-auto. auto.
-qed.
-local lemma yy &m : 
-  Pr[Y.main() @ &m : res] = 
-    Pr[Y2.main() @ &m : res].
-byequiv(_: ={glob D, glob V, glob P, glob Sim, glob HybOrcl} ==> _).
-proc. 
-unroll {1} 5.
-seq 6 6 : (={summary, glob V}).
-sim. call D_guess_prop. skip. auto.
-auto. auto.
-qed.
-local lemma ww &m : 
-  Pr[Z.main() @ &m : res] = 
-    Pr[Z2.main() @ &m : res].
-byequiv(_: ={glob D, glob V, glob P, glob Sim, glob HybOrcl} ==> _).
-proc. 
-unroll {1} 5.
-seq 6 6 : (={summary, glob V}).
-sim.
-call D_guess_prop. skip. auto.
-auto. auto.
-qed.
-lemma www &m : 
-  Pr[HybGame(A,Ob,L(Ob)).main() @ &m : res] = 
-  Pr[Z.main() @ &m : res].
-byequiv(_: ={glob D, glob V, glob P, glob Sim} ==> _).
-proc.
-inline {1} A(Ob, HybOrcl(Ob, L(Ob))).main.
-splitwhile {1} 5 : (i < HybOrcl.l0).
-seq 5 4 : (={glob V, glob P, HybOrcl.l, HybOrcl.l0, glob V, glob P, glob Sim, summary} /\
-  i{1} = HybOrcl.l{2} /\ HybOrcl.l0{2} <= HybOrcl.l{2}).
-simplify.
-while (={glob V, glob P, HybOrcl.l, HybOrcl.l0, glob V, glob P, glob Sim, summary} /\
-  i{1} = HybOrcl.l{2}). inline*.
-sp.
-rcondf {1} 1 . progress. skip.   progress.  smt.
-rcondf {2} 1 . progress. skip.   progress.  smt.
-rcondf {1} 1 . progress. skip.   progress.  smt.
-rcondf {2} 1 . progress. skip.   progress.  smt.
-sp. wp.  call (_:true). call (_:true). call (_:true). call (_:true).
-skip. progress.
-wp. rnd. skip. progress. smt.
-wp. 
-seq 1 1 : (={summary, glob V}).
-while (={glob V, glob P, HybOrcl.l, HybOrcl.l0, glob V, glob P, glob Sim, summary} /\
-  i{1} = HybOrcl.l{2} /\ HybOrcl.l0{2} <= HybOrcl.l{2} ). 
-wp. simplify. 
-inline HybOrcl(Ob, L(Ob)).orcl.
-wp. sp. if. progress. inline*. wp. 
-call (_: ={glob V}). sim. sim. sim. sim. 
-wp. skip. progress. smt. smt. 
-rcondt {1} 1. progress. skip. progress. smt.
-rcondt {2} 1. progress. skip. progress. smt.
-inline*. wp.
-call (_: ={glob V}). sim. sim. sim. sim. 
-wp.  skip. progress. smt. smt.  
-skip. progress.  
-call D_guess_prop. skip. auto.
-auto.
-auto.
-qed.
-lemma yyy &m : 
-  Pr[HybGame(A,Ob,R(Ob)).main() @ &m : res] = 
-  Pr[Y.main() @ &m : res].
-byequiv(_: ={glob D, glob V, glob P, glob Sim} ==> _).
-proc.
-inline {1} A(Ob, HybOrcl(Ob, R(Ob))).main.
-splitwhile {1} 5 : (i < HybOrcl.l0).
-seq 5 4 : (={glob V, glob P, HybOrcl.l, HybOrcl.l0, glob V, glob P, glob Sim, summary} /\
-  i{1} = HybOrcl.l{2} /\ HybOrcl.l0{2} <= HybOrcl.l{2}).
-simplify.
-while (={glob V, glob P, HybOrcl.l, HybOrcl.l0, glob V, glob P, glob Sim, summary} /\
-  i{1} = HybOrcl.l{2}). inline*.
-sp.
-rcondf {1} 1 . progress. skip.   progress.  smt.
-rcondf {2} 1 . progress. skip.   progress.  smt.
-rcondf {1} 1 . progress. skip.   progress.  smt.
-rcondf {2} 1 . progress. skip.   progress.  smt.
-sp. wp.  call (_:true). call (_:true). call (_:true). call (_:true).
-skip. progress.
-wp. rnd. skip. progress. smt.
-wp. 
-seq 1 1 : (={summary, glob V, glob HybOrcl}).
-while (={glob V, glob P, HybOrcl.l, HybOrcl.l0, glob V, glob P, glob Sim, summary} /\
-  i{1} = HybOrcl.l{2} /\ HybOrcl.l0{2} <= HybOrcl.l{2} ). 
-wp. simplify. 
-inline HybOrcl(Ob, R(Ob)).orcl.
-wp. sp. if. progress. inline*. wp. 
-call (_: ={glob V, glob HybOrcl}). sim. sim. sim. sim. 
-wp. skip. progress. smt. smt. 
-rcondt {1} 1. progress. skip. progress. smt.
-rcondt {2} 1. progress. skip. progress. smt.
-inline*. wp. sp.  call (_:true). call (_:true). call (_:true). call (_:true).
-skip. progress. smt. smt.
-skip. progress.  call D_guess_prop. skip. auto.
-auto.
-auto.
-qed.
-lemma qq &m:
-        Pr[Ln(Ob,A).main() @ &m : res]
-      - Pr[Rn(Ob,A).main() @ &m : res]
-    = n%r *(Pr[HybGame(A,Ob,L(Ob)).main() @ &m : res]
-            - Pr[HybGame(A,Ob,R(Ob)).main() @ &m : res]).
-apply (Hybrid_restr Ob A _ _ _ _ _ &m (fun _ _ _ r => r)).
-progress. proc. inline*.
-wp.  call (_:true). 
-while (Count.c = i /\ i <= n) . wp. 
-call (_:true). wp.  skip.  progress. smt.
-wp.  skip.  progress. smt.
-proc. skip. auto. proc.
-call (sim_run_ll V). apply V_challenge_ll.
-apply V_summitup_ll. skip. auto.
-proc. call V_summitup_ll. call P_response_ll.
-call V_challenge_ll. call P_commitment_ll. skip. auto.
-progress.
-proc. call D_guess_ll. sp.
-while (true) (n - i + 1). progress.
-wp. call H. skip. progress. smt.
-progress. skip. progress. smt.
-qed.
-
-
-
-module Ob1 = Obb(P,V,Sim).
-module A1 = Ad(D).
-
-module Amem : IR1R2 = {
-  proc init() = {
-   var commit, challenge, response, summary;
-   HybOrcl.l0 <$ [0..max 0 (n -1 )];
-   HybOrcl.l <- 0;
-   summary <- witness;
-   while (HybOrcl.l < n && HybOrcl.l < HybOrcl.l0) {
-     commit <@ P.commitment(s, w);
-     challenge <@ V.challenge(s, commit);
-     response <@ P.response(challenge);
-     summary <@ V.summitup(s, response);
-     HybOrcl.l <- HybOrcl.l + 1;
-   }
-  }
-  proc run1() = {
-   var  summary, guess;
-   summary <@ Sim(V).simulate(s);
-   HybOrcl.l <- HybOrcl.l + 1;
-   while (HybOrcl.l < n) {
-    summary <@ Sim(V).simulate(s);
-    HybOrcl.l <- HybOrcl.l + 1;
-   }
-   guess <@ D.guess(s, w, summary);
-   return guess;
-  }
-  proc run2() = {
-   var commit, challenge, response, summary, guess;
-   commit <@ P.commitment(s, w);
-   challenge <@ V.challenge(s, commit);
-   response <@ P.response(challenge);
-   summary <@ V.summitup(s, response);
-   HybOrcl.l <- HybOrcl.l + 1;
-   while (HybOrcl.l < n) {
-    summary <@ Sim(V).simulate(s);
-    HybOrcl.l <- HybOrcl.l + 1;
-   }
-   guess <@ D.guess(s, w, summary);
-   return guess;
-  }
-}.
-
-module Dstar : ZKDistinguisher = {
-  proc guess(ss : statement, ww: witness, summary: adv_summary) = {
-   var guess;
-   HybOrcl.l <- HybOrcl.l + 1;
-   while (HybOrcl.l < n) {
-    summary <@ Sim(V).simulate(s);
-    HybOrcl.l <- HybOrcl.l + 1;
-   }
-   guess <@ D.guess(s, w,  summary);
-   return guess;
-  }
-}.
-
-
-local lemma lll &m deltoid : 
-   (forall &n,
-   Pr[ZKIdeal(Sim, V, Dstar).run(s, w) @ &n : res]
-    - Pr[ZKReal(P, V, Dstar).run(s, w) @ &n : res] 
-           < deltoid) =>
-   Pr[HybGame(A1,Ob1,L(Ob1)).main() @ &m : res]
-               - Pr[HybGame(A1,Ob1,R(Ob1)).main() @ &m : res] < deltoid.
-move => zk_ass.
-have ->: Pr[HybGame(A1,Ob1,L(Ob1)).main() @ &m : res] =
-         Pr[MemoryPropsLE.P(Amem).main1() @ &m : res].
-rewrite www. rewrite ww. rewrite w.
-byequiv. proc. 
-inline Amem.run1. inline Amem.init.
-wp.  seq 7 7 : (={summary, glob V}). sim. smt.
-call D_guess_prop. skip. auto.
-auto. auto.
-have ->: Pr[HybGame(A1,Ob1,R(Ob1)).main() @ &m : res] =
-         Pr[MemoryPropsLE.P(Amem).main2() @ &m : res].
-rewrite yyy. rewrite yy. rewrite y.
-byequiv. proc. 
-inline Amem.run2. inline Amem.init.
-wp. seq 10 10 : (={summary, glob V}). sim. smt. 
-call D_guess_prop. skip. auto.
-auto. auto.
-case (Pr[MemoryPropsLE.P(Amem).main1() @ &m : res] -
-Pr[MemoryPropsLE.P(Amem).main2() @ &m : res] < deltoid). auto.
-move => q.
-have zz : Pr[MemoryPropsLE.P(Amem).main1() @ &m : res] -
-  Pr[MemoryPropsLE.P(Amem).main2() @ &m : res] >= deltoid. 
-smt. clear q.
-have ko : exists &n, deltoid <= Pr[Amem.run1() @ &n : res] - Pr[Amem.run2() @ &n : res].
-apply (o_o Amem &m).  auto.
-elim ko. move => &n. move => q.
-have ok : Pr[Amem.run1() @ &n : res] - Pr[Amem.run2() @ &n : res] < deltoid.
-have -> : Pr[Amem.run1() @ &n : res] = Pr[ZKIdeal(Sim, V, Dstar).run(s, w) @ &n : res].
-byequiv. proc.         
-inline Dstar.guess. wp.
-seq 3 6: (={glob V} /\ summary{1} = summary0{2}). sim. wp.
-call (_: ={glob V}). sim. sim. sim. sim. skip. progress. 
-smt. smt.
-call D_guess_prop. skip. auto.
-auto.  auto. 
-have -> : Pr[Amem.run2() @ &n : res] = Pr[ZKReal(P, V, Dstar).run(s, w) @ &n : res].
-byequiv. proc.         
-inline Dstar.guess. wp.
-seq 6 9: (={glob V} /\ summary{1} = summary0{2}). sim. wp.
-call (_:true). call (_:true).  call (_:true).  call (_:true). skip.
-progress. smt. smt. smt.  call D_guess_prop. skip. auto.
-auto.  auto. 
-apply (zk_ass  &n ). smt. 
-qed.
-
-
-
-
-lemma zk_seq &m deltoid : 
-   (forall &n,
-   Pr[ZKIdeal(Sim, V, Dstar).run(s, w) @ &n : res]
-    - Pr[ZKReal(P, V, Dstar).run(s, w) @ &n : res] 
-           < deltoid) =>
-
-   Pr[ZKIdeal(SimAmp(Sim), V, D).run(s, w) @ &m : res]
-        - Pr[ZKRealAmp(P, V, D).run(s, w) @ &m : res]
-          < n%r * deltoid.
-move => zk_ass.
-have -> : Pr[ZKIdeal(SimAmp(Sim), V, D).run(s, w) @ &m : res]
- = Pr[Ln(Ob,A).main() @ &m : res].
-byequiv (_:   
-  (glob V){2} = (glob V){m} /\ ={glob Sim}/\
-  (statement{1}, witness{1}, n{1}) = (s, w, n) /\
-   (glob V){1} = (glob V){m} ==> _). proc. inline*. wp. sp.
-seq 2 1 : (={glob V, summary} /\ statement{1} = s{2} /\ witness{1} = w{2}).   simplify. wp.
-while (={i, glob V, glob Sim} /\ summary0{1} = summary{2} /\ statement0{1} = s ).
-wp. call (_: ={glob V}). sim. sim. sim. sim. wp.  skip. progress.
- skip. progress.  call D_guess_prop. skip. auto. auto. auto.
-have -> : Pr[ZKRealAmp(P, V, D).run(s, w) @ &m : res]
- = Pr[Rn(Ob,A).main() @ &m : res].
-byequiv (_: ={glob V, glob P} /\ (statement{1}, witness{1}) = (s, w) ==> _). proc.
-inline*. wp. sp.
-seq 1 1 : (={glob V, summary} /\ statement{1} = s{2} /\ witness{1} = w{2} ).   simplify. wp.
-while (={i, glob V, glob P} /\ summary{1} = summary{2} /\ statement{1} = s /\  witness{1} = w{2}). sp. wp.
-call (_:true). call (_:true). call (_:true). call (_:true). skip. progress.
-skip. progress. call D_guess_prop. skip.  auto. auto. auto.
-rewrite qq.
-have :  Pr[HybGame(A1,Ob1,L(Ob1)).main() @ &m : res]
-               - Pr[HybGame(A1,Ob1,R(Ob1)).main() @ &m : res] < deltoid.
-apply lll. smt. smt.
-qed.
-
-
-end section.
-
-end SequentialCompositionZK.
-
 
