memory_props/MemoryPropsLE.ec
@@ -5,8 +5,10 @@ require import AllCore Distr DBool.
 require import Reflection ReflectionComp.
 require WholeMsg.
 
-clone import ReflComp with type at1 <- unit,
-                           type at2 <- unit,
+type at2, at1.
+
+clone import ReflComp with type at1 <- at1,
+                           type at2 <- at2,
                            type rt1 <- unit,
                            type rt2 <- bool.
 
@@ -39,59 +41,59 @@ qed.
 
 
 lemma www &m p :   
-    exists (D1 : unit -> (glob A) -> (unit * (glob A)) distr)
-      (D2 : unit -> unit * (glob A) -> (glob A) distr),
-      (forall &m (M : unit * (glob A) -> bool),
-         mu (D1 tt (glob A){m}) M = Pr[A.ex1() @ &m : M (res, (glob A))]) /\
-      (forall &m (M : (glob A) -> bool) (r1 i2 : unit),
+    exists (D1 : at1 -> (glob A) -> (unit * (glob A)) distr)
+      (D2 : at2 -> unit * (glob A) -> (glob A) distr),
+      (forall &m (M : unit * (glob A) -> bool) i1,
+         mu (D1 i1 (glob A){m}) M = Pr[A.ex1(i1) @ &m : M (res, (glob A))]) /\
+      (forall &m (M : (glob A) -> bool) (r1 : unit) i2,
          mu (D2 i2 (r1, (glob A){m})) M =
          Pr[A.ex2(i2, r1) @ &m : M (glob A)]) /\
-      (forall &m (M : (glob A) -> bool) (i1 i2 : unit),
+      (forall &m (M : (glob A) -> bool)  i1 i2,
         mu ((dlet (D1 i1 (glob A){m}) (D2 i2))) M =
         Pr[RCR(A).main(i1, i2) @ &m : M (glob A)]) 
-   /\ forall (M :  (glob A) -> bool), 
-       p <= Pr[ RCR(A).main(tt,tt) @ &m : M (glob A) ]  =>
+   /\ forall (M :  (glob A) -> bool) i1 i2, 
+       p <= Pr[ RCR(A).main(i1,i2) @ &m : M (glob A) ]  =>
        0%r < p =>
-   exists g, 0%r < mu1 (D1 tt (glob A){m}) (tt,g)  /\ mu (D2 tt ((tt,g))) M >= p.
+   exists g, 0%r < mu1 (D1 i1 (glob A){m}) (tt,g)  /\ mu (D2 i2 ((tt,g))) M >= p.
 proof.  elim (refl_comp_simple A). progress.
-exists D1 D2. progress. rewrite H. auto.
+exists D1 D2. progress.
 pose g0 := (glob A){m}.
 case (exists (g : (glob A)),
-  0%r < mu1 (D1 tt g0) (tt, g) /\ p <= mu (D2 tt (tt, g)) M).
+  0%r < mu1 (D1 i1 g0) (tt, g) /\ p <= mu (D2 i2 (tt, g)) M).
 auto.
 move => G.
 have: (forall (g : (glob A)),
-     ! (0%r < mu1 (D1 tt g0) (tt, g) /\ p <= mu (D2 tt (tt, g)) M)).
+     ! (0%r < mu1 (D1 i1 g0) (tt, g) /\ p <= mu (D2 i2 (tt, g)) M)).
 smt.
 clear G.
 move => G.
-have q : forall (g : glob A),  mu1 (D1 tt g0) (tt,g) > 0%r => mu (D2 tt (tt,g)) M < p .
+have q : forall (g : glob A),  mu1 (D1 i1 g0) (tt,g) > 0%r => mu (D2 i2 (tt,g)) M < p .
 smt.
-have q2 : exists g, 0%r < mu1 (D1 tt g0) (tt, g).
-case (exists (g : (glob A)), 0%r < mu1 (D1 tt g0) (tt, g)). auto.
+have q2 : exists g, 0%r < mu1 (D1 i1 g0) (tt, g).
+case (exists (g : (glob A)), 0%r < mu1 (D1 i1 g0) (tt, g)). auto.
 move => q21.
-have q22  : forall (g : (glob A)), 0%r = mu1 (D1 tt g0) (tt, g).
+have q22  : forall (g : (glob A)), 0%r = mu1 (D1 i1 g0) (tt, g).
 smt. clear q21.
-have : Pr[RCR(A).main(tt, tt) @ &m : true ] = 0%r.
+have : Pr[RCR(A).main(i1, i2) @ &m : true ] = 0%r.
 rewrite -  (H1 &m predT). 
 rewrite dlet_mu_main. 
 apply sum0_eq. progress. 
  have -> : x = (tt, x.`2). smt.
 rewrite - q22. smt. smt.
 elim q2. move => g gp.
-have : mu (dlet (D1 tt (glob A){m}) (D2 tt)) M < p.
+have : mu (dlet (D1 i1 (glob A){m}) (D2 i2)) M < p.
 rewrite  dlet_mu_main.
 rewrite (sum_split _ (pred1 (tt, g))). 
-apply (summable_mu1_wght ((D1 tt (glob A){m})) (fun x => mu (D2 tt x) M)   _) .
+apply (summable_mu1_wght ((D1 i1 (glob A){m})) (fun x => mu (D2 i2 x) M)   _) .
 smt.
 simplify.
 have -> : sum
   (fun (x : unit * (glob A)) =>
-     if  pred1 (tt, g) x then mu1 (D1 tt (glob A){m}) x * mu (D2 tt x) M
-     else 0%r) = mu1 (D1 tt (glob A){m}) (tt,g) * mu (D2 tt (tt,g)) M.
+     if  pred1 (tt, g) x then mu1 (D1 i1 (glob A){m}) x * mu (D2 i2 x) M
+     else 0%r) = mu1 (D1 i1 (glob A){m}) (tt,g) * mu (D2 i2 (tt,g)) M.
   have ->: (fun (x : unit * (glob A)) =>
-     if  pred1 (tt, g) x then mu1 (D1 tt (glob A){m}) x * mu (D2 tt x) M
-     else 0%r) = (fun (x : unit * (glob A)) => mu1 (D1 tt (glob A){m}) (tt,g) * mu (D2 tt (tt,g)) M *
+     if  pred1 (tt, g) x then mu1 (D1 i1 (glob A){m}) x * mu (D2 i2 x) M
+     else 0%r) = (fun (x : unit * (glob A)) => mu1 (D1 i1 (glob A){m}) (tt,g) * mu (D2 i2 (tt,g)) M *
      if  pred1 (tt, g) x then (mu1 (duniform [(tt,g)]) x)
      else 0%r).
 apply fun_ext. move => x.  
@@ -104,75 +106,75 @@ rewrite - muE. progress.
 have ->: mu1 (duniform [(tt, g)]) (tt, g) = 1%r. smt. smt.
 have zzz : sum
   (fun (x : unit * (glob A)) =>
-     if ! pred1 (tt, g) x then mu1 (D1 tt (glob A){m}) x * mu (D2 tt x) M
+     if ! pred1 (tt, g) x then mu1 (D1 i1 (glob A){m}) x * mu (D2 i2 x) M
      else 0%r) <= sum
   (fun (x : unit * (glob A)) =>
-     if ! pred1 (tt, g) x then mu1 (D1 tt (glob A){m}) x * p
+     if ! pred1 (tt, g) x then mu1 (D1 i1 (glob A){m}) x * p
      else 0%r).
 apply ler_sum. progress. 
 case (pred1 (tt, g) x). simplify. auto. simplify. progress.
 have ->: x = (tt,x.`2). smt.
-case (mu1 (D1 tt (glob A){m}) (tt, x.`2) = 0%r). 
+case (mu1 (D1 i1 (glob A){m}) (tt, x.`2) = 0%r). 
 smt.
 smt.
 have ->: (fun (x : unit * (glob A)) =>
-     if ! pred1 (tt, g) x then mu1 (D1 tt (glob A){m}) x * mu (D2 tt x) M
-     else 0%r) = (fun (x : unit * (glob A)) => mu1 (D1 tt (glob A){m}) x * 
-     if ! pred1 (tt, g) x then mu (D2 tt x) M
+     if ! pred1 (tt, g) x then mu1 (D1 i1 (glob A){m}) x * mu (D2 i2 x) M
+     else 0%r) = (fun (x : unit * (glob A)) => mu1 (D1 i1 (glob A){m}) x * 
+     if ! pred1 (tt, g) x then mu (D2 i2 x) M
      else 0%r).
 apply fun_ext. move => x. smt.
 apply summable_mu1_wght. progress. smt. smt.
 have -> : (fun (x : unit * (glob A)) =>
-     if ! pred1 (tt, g) x then mu1 (D1 tt (glob A){m}) x * p else 0%r)
+     if ! pred1 (tt, g) x then mu1 (D1 i1 (glob A){m}) x * p else 0%r)
  = (fun (x : unit * (glob A)) => p *
-     if ! pred1 (tt, g) x then mu1 (D1 tt (glob A){m}) x else 0%r).
+     if ! pred1 (tt, g) x then mu1 (D1 i1 (glob A){m}) x else 0%r).
 apply fun_ext. move => x. smt.
 apply summableZ.
 have ->: (fun (x : unit * (glob A)) =>
-     if ! pred1 (tt, g) x then mu1 (D1 tt (glob A){m}) x else 0%r)
- = (fun (x : unit * (glob A)) => mu1 (D1 tt (glob A){m}) x *
+     if ! pred1 (tt, g) x then mu1 (D1 i1 (glob A){m}) x else 0%r)
+ = (fun (x : unit * (glob A)) => mu1 (D1 i1 (glob A){m}) x *
      if ! pred1 (tt, g) x then 1%r else 0%r).
 smt.
 apply summable_mu1_wght. progress. smt. smt.
-have : mu1 (D1 tt (glob A){m}) (tt, g) * mu (D2 tt (tt, g)) M +
+have : mu1 (D1 i1 (glob A){m}) (tt, g) * mu (D2 i2 (tt, g)) M +
 sum
   (fun (x : unit * (glob A)) =>
-     if ! pred1 (tt, g) x then mu1 (D1 tt (glob A){m}) x * p
+     if ! pred1 (tt, g) x then mu1 (D1 i1 (glob A){m}) x * p
      else 0%r) < p.
-apply (ler_trans1 _ (mu1 (D1 tt (glob A){m}) (tt, g) * p +
+apply (ler_trans1 _ (mu1 (D1 i1 (glob A){m}) (tt, g) * p +
 sum
   (fun (x : unit * (glob A)) =>
-     if ! pred1 (tt, g) x then mu1 (D1 tt (glob A){m}) x * p else 0%r) )  p _ _).
+     if ! pred1 (tt, g) x then mu1 (D1 i1 (glob A){m}) x * p else 0%r) )  p _ _).
 clear zzz G H H0 H1. 
-have : mu (D2 tt (tt, g)) M
+have : mu (D2 i2 (tt, g)) M
  <  p.
 smt.
 smt.
-have ->: mu1 (D1 tt (glob A){m}) (tt, g) * p +
+have ->: mu1 (D1 i1 (glob A){m}) (tt, g) * p +
  sum
   (fun (x : unit * (glob A)) =>
-     if ! pred1 (tt, g) x then mu1 (D1 tt (glob A){m}) x * p else 0%r)
+     if ! pred1 (tt, g) x then mu1 (D1 i1 (glob A){m}) x * p else 0%r)
   = sum
   (fun (x : unit * (glob A)) =>
-      mu1 (D1 tt (glob A){m}) x * p).
+      mu1 (D1 i1 (glob A){m}) x * p).
 search sum.
 print sumD1.
-rewrite (sumD1 (fun (x : unit * (glob A)) => mu1 (D1 tt (glob A){m}) x * p) (tt,g)). 
-have ->: (fun (x : unit * (glob A)) => mu1 (D1 tt (glob A){m}) x * p) 
- = (fun (x : unit * (glob A)) => p * mu1 (D1 tt (glob A){m}) x ).
+rewrite (sumD1 (fun (x : unit * (glob A)) => mu1 (D1 i1 (glob A){m}) x * p) (tt,g)). 
+have ->: (fun (x : unit * (glob A)) => mu1 (D1 i1 (glob A){m}) x * p) 
+ = (fun (x : unit * (glob A)) => p * mu1 (D1 i1 (glob A){m}) x ).
 smt.
 apply summableZ.
 apply summable_mu1.
 simplify. auto.
-have ->: sum (fun (x : unit * (glob A)) => mu1 (D1 tt (glob A){m}) x * p)
- = p * sum (fun (x : unit * (glob A)) => mu1 (D1 tt (glob A){m}) x).
+have ->: sum (fun (x : unit * (glob A)) => mu1 (D1 i1 (glob A){m}) x * p)
+ = p * sum (fun (x : unit * (glob A)) => mu1 (D1 i1 (glob A){m}) x).
 rewrite -  sumZ.   simplify.
- have ->: (fun (x : unit * (glob A)) => mu1 (D1 tt (glob A){m}) x * p) 
- = (fun (x : unit * (glob A)) => p * mu1 (D1 tt (glob A){m}) x).
+ have ->: (fun (x : unit * (glob A)) => mu1 (D1 i1 (glob A){m}) x * p) 
+ = (fun (x : unit * (glob A)) => p * mu1 (D1 i1 (glob A){m}) x).
 smt.
 auto.
-have ->: (fun (x : unit * (glob A)) => mu1 (D1 tt (glob A){m}) x)
- = (fun (x : unit * (glob A)) => if predT x then mu1 (D1 tt (glob A){m}) x else 0%r).
+have ->: (fun (x : unit * (glob A)) => mu1 (D1 i1 (glob A){m}) x)
+ = (fun (x : unit * (glob A)) => if predT x then mu1 (D1 i1 (glob A){m}) x else 0%r).
 smt.
 rewrite - muE.
 smt.
@@ -186,32 +188,32 @@ qed.
 lemma ZzZ &m M i1 i2 p: 
        p <= Pr[ RCR(A).main(i1,i2) @ &m : M (glob A) ] 
    => 0%r < p
-   => exists &n, p <= Pr[ A.ex2(tt, tt) @ &n  : M (glob A)] .
+   => exists &n, p <= Pr[ A.ex2(i2, tt) @ &n  : M (glob A)] .
 elim (www &m p). progress.
-elim (H2 M _ _);auto. smt. progress.
-have f1 : Pr[A.ex1() @ &m : glob A = g] > 0%r.
-have f2 : mu (D1 tt (glob A){m}) (fun x => snd x = g)  = Pr[A.ex1() @ &m : (glob A) = g].
+elim (H2 M i1 i2 _ _);auto. progress.
+have f1 : Pr[A.ex1(i1) @ &m : glob A = g] > 0%r.
+have f2 : mu (D1 i1 (glob A){m}) (fun x => snd x = g)  = Pr[A.ex1(i1) @ &m : (glob A) = g].
 rewrite (H &m ). auto. smt. 
 have f3: exists &n, g = (glob A){n}.
-  have  f31: Pr[A.ex1() @ &m : (glob A) = g /\ (exists &n, (glob A) = (glob A){n}) ] = Pr[A.ex1() @ &m : (glob A) = g].
-  have <- : Pr[A.ex1() @ &m : (glob A) = g] = Pr[A.ex1() @ &m : (glob A) = g /\ exists &n, (glob A) = (glob A){n}].
+  have  f31: Pr[A.ex1(i1) @ &m : (glob A) = g /\ (exists &n, (glob A) = (glob A){n}) ] = Pr[A.ex1(i1) @ &m : (glob A) = g].
+  have <- : Pr[A.ex1(i1) @ &m : (glob A) = g] = Pr[A.ex1(i1) @ &m : (glob A) = g /\ exists &n, (glob A) = (glob A){n}].
   rewrite Pr[mu_split exists &n, (glob A) = (glob A){n}].
-  have : Pr[A.ex1() @ &m : (glob A) = g /\ ! (exists &n, (glob A) = (glob A){n})] = 0%r. smt. smt. auto.
-  have f32 : Pr[A.ex1() @ &m : (glob A) = g /\ exists &n, g = (glob A){n}] =
-     Pr[A.ex1() @ &m : (glob A) = g].
+  have : Pr[A.ex1(i1) @ &m : (glob A) = g /\ ! (exists &n, (glob A) = (glob A){n})] = 0%r. smt. smt. auto.
+  have f32 : Pr[A.ex1(i1) @ &m : (glob A) = g /\ exists &n, g = (glob A){n}] =
+     Pr[A.ex1(i1) @ &m : (glob A) = g].
   rewrite - f31. rewrite Pr[mu_eq]. progress. auto.
-  have f33 : Pr[A.ex1() @ &m : exists &n, g = (glob A){n}] > 0%r.
-         have f331 : Pr[A.ex1() @ &m : (glob A) = g /\ exists &n, (glob A) = (glob A){n}] 
-                         <= Pr[A.ex1() @ &m : (glob A) = g]. smt.
+  have f33 : Pr[A.ex1(i1) @ &m : exists &n, g = (glob A){n}] > 0%r.
+         have f331 : Pr[A.ex1(i1) @ &m : (glob A) = g /\ exists &n, (glob A) = (glob A){n}] 
+                         <= Pr[A.ex1(i1) @ &m : (glob A) = g]. smt.
        smt.
   clear f32 f31 f1    H2 H1 H0 H. 
   case (exists &n, g = (glob A){n}). auto.
   move => q. 
-   have : Pr[A.ex1() @ &m : exists &n, g = (glob A){n}] = Pr[A.ex1() @ &m : false]. 
+   have : Pr[A.ex1(i1) @ &m : exists &n, g = (glob A){n}] = Pr[A.ex1(i1) @ &m : false]. 
    rewrite Pr[mu_eq]. progress. auto. smt.
 elim f3. progress.
 exists &n.
-rewrite -  (H0 &n M tt tt). auto.
+rewrite -  (H0 &n M tt i2). auto.
 qed.
 
 
@@ -227,8 +229,8 @@ declare axiom A_run_ll : islossless A.ex1.
 local module A' = {
   var r : bool
   proc ex1 = A.ex1
-  proc ex2(x:unit*unit) = {
-    r <@ A.ex2(tt,tt);
+  proc ex2(x:at2*unit) = {
+    r <@ A.ex2(x);
     return r;
   }
 
@@ -236,7 +238,7 @@ local module A' = {
 
 lemma ZzZ_res &m M i1 i2 p: 
        p <= Pr[ RCR(A).main(i1,i2) @ &m : M res.`2 ] 
-   => exists &n, p <= Pr[ A.ex2(tt, tt) @ &n  : M res] .
+   => exists &n, p <= Pr[ A.ex2(i2, tt) @ &n  : M res] .
 
 
 case (p <= 0%r).  progress. exists &m. smt.
@@ -249,12 +251,12 @@ have -> : Pr[ RCR(A).main(i1,i2) @ &m : M res.`2 ]  = Pr[ RCR(A').main(i1,i2) @ 
 byequiv. proc. inline*.
 wp.  call (_:true). wp.  call (_:true). skip. auto. auto. auto.
 progress.
-have f : exists &n, p <= Pr[ A'.ex2(tt, tt) @ &n  : M A'.r ] .
+have f : exists &n, p <= Pr[ A'.ex2(i2, tt) @ &n  : M A'.r ] .
 apply (ZzZ A' _ &m (fun (x : glob A') => M x.`1) i1 i2 p). 
 proc*. call A_run_ll. skip. auto. simplify.  apply H. auto. 
 elim f. progress. exists &n.
-have <-: Pr[A'.ex2(tt, tt) @ &n : M A'.r] = 
-  Pr[A.ex2(tt, tt) @ &n : M res]. 
+have <-: Pr[A'.ex2(i2, tt) @ &n : M A'.r] = 
+  Pr[A.ex2(i2, tt) @ &n : M res]. 
 byequiv.  proc*. inline*. sp.  wp. call (_:true). skip. auto. auto.
 auto. auto.
 qed.
@@ -263,49 +265,49 @@ end section.
    
 
 module type IR1R2 = {
-  proc init() : unit
-  proc run1() : bool
-  proc run2() : bool
+  proc init(i1:at1) : unit
+  proc run1(i2:at2) : bool
+  proc run2(i2:at2) : bool
 }.
 
 module P(A : IR1R2) = {
-  proc main1() = {
+  proc main1(i1:at1,i2:at2) = {
     var r : bool;
-    A.init();
-    r <@ A.run1();
+    A.init(i1);
+    r <@ A.run1(i2);
     return r;
   }
 
-  proc main2() = {
+  proc main2(i1:at1,i2:at2) = {
     var r : bool;
-    A.init();
-    r <@ A.run2();
+    A.init(i1);
+    r <@ A.run2(i2);
     return r;
   }
 
-  proc init_main12() = {
+  proc init_main12(i1:at1,i2:at2) = {
    var b, r', r : bool;
 
-   A.init();
+   A.init(i1);
    b <$ {0,1};
    
    if(b){
-     r <@ A.run1();
+     r <@ A.run1(i2);
    }else{
-     r' <@ A.run2();
+     r' <@ A.run2(i2);
      r  <- !r';
    }
    return r;
   }
 
-  proc main12() = {
+  proc main12(i2:at2) = {
    var b, r', r : bool;
    b <$ {0,1};
    
    if(b){
-     r <@ A.run1();
+     r <@ A.run1(i2);
    }else{
-     r' <@ A.run2();
+     r' <@ A.run2(i2);
      r  <- !r';
    }
    return r;
@@ -353,38 +355,38 @@ smt.
 qed.
 
 local module A'' = {
-  proc ex1() = { 
-     A.init();
+  proc ex1(i1:at1) = { 
+     A.init(i1);
   }
 
-  proc ex2(x:unit*unit) = {
+  proc ex2(x:at2*unit) = {
      var r;
-     r <@ P(A).main12()     ;
+     r <@ P(A).main12(x.`1)     ;
      return r;
   }
 }.
 
 
-lemma d_b3 &m p M : p <= Pr[ P(A).init_main12() @ &m : M res ] 
-   => exists &n, p <= Pr[ P(A).main12() @ &n : M  res ].
+lemma d_b3 &m p M ii1 ii2 : p <= Pr[ P(A).init_main12(ii1,ii2) @ &m : M res ] 
+   => exists &n, p <= Pr[ P(A).main12(ii2) @ &n : M  res ].
 have ->: 
-  Pr[ P(A).init_main12() @ &m : M res ]
-  =  Pr[RCR(A'').main(tt,tt) @ &m : M res.`2 ] .
+  Pr[ P(A).init_main12(ii1,ii2) @ &m : M res ]
+  =  Pr[RCR(A'').main(ii1,ii2) @ &m : M res.`2 ] .
 byequiv. proc. inline*. wp. simplify. inline A''.ex1.
-sp.  seq 2 3 : (={glob A, b}). rnd.  wp. call (_:true). skip.
+sp.  seq 2 4 : (={glob A, b,i1} /\ i2{1} = i20{2}). rnd.  wp. call (_:true). skip.
 progress. if. auto. call (_:true). skip.  auto.
 wp.  call (_:true). skip.  auto. auto. auto. 
 progress.
-have : exists &n, p <= Pr[ A''.ex2(tt, tt) @ &n  : M res].
-apply (ZzZ_res A'' _ &m M tt tt p). 
+have : exists &n, p <= Pr[ A''.ex2(ii2, tt) @ &n  : M res].
+apply (ZzZ_res A'' _ &m M ii1 ii2 p). 
 proc. call A_init_ll. skip. auto.
 auto. 
 elim. progress.
 exists &n. 
-have ->: Pr[P(A).main12() @ &n : M res]
- = Pr[A''.ex2(tt, tt) @ &n : M res].
+have ->: Pr[P(A).main12(ii2) @ &n : M res]
+ = Pr[A''.ex2(ii2, tt) @ &n : M res].
 byequiv. proc.  inline*. wp. sp. 
-seq 1 1 : (={glob A, b}). rnd. skip. auto.
+seq 1 1 : (={glob A, b,i2}). rnd. skip. auto.
  if. auto. call (_:true). skip.  auto.
 wp.  call (_:true). skip.  auto. auto. auto. 
 progress.
@@ -394,19 +396,19 @@ qed.
 clone import WholeMsg as WM with type message <- bool,
                             op m1 <- false,
                             op m2 <- true,
-                            type ain <- unit.
+                            type ain <- at1*at2.
 
 
 
 local module T = {
-  proc main(b:bool, t:unit) = {
+  proc main(b:bool, i1i2:at1*at2) = {
    var r', r : bool;
 
-   A.init();   
+   A.init(i1i2.`1);   
    if(b){
-     r <@ A.run1();
+     r <@ A.run1(i1i2.`2);
    }else{
-     r' <@ A.run2();
+     r' <@ A.run2(i1i2.`2);
      r  <- !r';
    }
    return r;
@@ -414,13 +416,13 @@ local module T = {
 }.
 
 local module T2 = {
-  proc main(b:bool, t:unit) = {
+  proc main(b:bool, i1i2:at1*at2) = {
    var r', r : bool;
 
    if(b){
-     r <@ A.run1();
+     r <@ A.run1(i1i2.`2);
    }else{
-     r' <@ A.run2();
+     r' <@ A.run2(i1i2.`2);
      r  <- !r';
    }
    return r;
@@ -431,29 +433,37 @@ local module T2 = {
 
 
 
-lemma d_b1 &m : Pr[ P(A).init_main12() @ &m : res ] 
-  = f (Pr[ P(A).main1() @ &m : res ] - Pr[ P(A).main2() @ &m : res ]) .
-have ->: Pr[ P(A).init_main12() @ &m : res ] 
- = Pr[ W(T).main() @ &m : res ].
-byequiv (_: ={glob A} ==> _). proc. inline*. swap {1} 2 -1. sim. 
-rnd. skip. smt. auto. auto.
+lemma d_b1 ii1 ii2 &m : Pr[ P(A).init_main12(ii1,ii2) @ &m : res ] 
+  = f (Pr[ P(A).main1(ii1,ii2) @ &m : res ] - Pr[ P(A).main2(ii1,ii2) @ &m : res ]) .
+have ->: Pr[ P(A).init_main12(ii1,ii2) @ &m : res ] 
+ = Pr[ W(T).main(ii1,ii2) @ &m : res ].
+byequiv (_: ={glob A} /\ (i1,i2){1} = a{2} /\  (ii1,ii2) = a{2} ==> _). proc. inline*. swap {1} 2 -1. simplify.
+
+seq 2 4 :( ={b,glob A} /\ (i1,i2){1} = i1i2{2} ).  call (_:true). 
+wp.  rnd. skip. progress. smt. smt.
+if. auto. wp. call (_:true). skip. auto.
+wp. call (_:true). skip. auto. auto. auto.
+
 rewrite (splitcases T).
-have ->: Pr[T.main(false, tt) @ &m : res] 
- = Pr[ P(A).main2() @ &m : !res ].
+have ->: Pr[T.main(false, (ii1,ii2)) @ &m : res] 
+ = Pr[ P(A).main2(ii1,ii2) @ &m : !res ].
 byequiv. proc. rcondf {1} 2. progress. call (_:true).
 skip.  smt.
-wp.   sim. auto. auto.
-have ->: Pr[T.main(true, tt) @ &m : res] 
- = Pr[ P(A).main1() @ &m : res ].
+wp.   sim.  call (_:true). call (_:true).  skip. auto. auto. auto.
+
+have ->: Pr[T.main(true, (ii1,ii2)) @ &m : res] 
+ = Pr[ P(A).main1(ii1,ii2) @ &m : res ].
 byequiv. proc. rcondt {1} 2. progress. call (_:true).
 skip.  smt.
-wp.   sim. auto. auto.
+wp.
+call (_:true). call (_:true).  skip. auto. auto. auto.
+
 rewrite /f.
-have -> : (1%r + (Pr[P(A).main1() @ &m : res] - Pr[P(A).main2() @ &m : res]))
- = Pr[P(A).main1() @ &m : res] + (1%r - Pr[P(A).main2() @ &m : res]).
+have -> : (1%r + (Pr[P(A).main1(ii1,ii2) @ &m : res] - Pr[P(A).main2(ii1,ii2) @ &m : res]))
+ = Pr[P(A).main1(ii1,ii2) @ &m : res] + (1%r - Pr[P(A).main2(ii1,ii2) @ &m : res]).
 smt.
-have ->: (1%r - Pr[P(A).main2() @ &m : res]) = Pr[P(A).main2() @ &m : !res].
-   have -> : 1%r = Pr[P(A).main2() @ &m : true].
+have ->: (1%r - Pr[P(A).main2(ii1,ii2) @ &m : res]) = Pr[P(A).main2(ii1,ii2) @ &m : !res].
+   have -> : 1%r = Pr[P(A).main2(ii1,ii2) @ &m : true].
  byphoare. proc. call A_run2_ll. call A_init_ll. skip.  auto. auto. auto.
 rewrite Pr[mu_split res]. simplify. smt.
 smt.
@@ -461,30 +471,38 @@ qed.
 
 
 
-lemma d_b2 &m : Pr[ P(A).main12() @ &m : res ] 
-  = f (Pr[ A.run1() @ &m : res ] - Pr[ A.run2() @ &m : res ]) .
-have ->: Pr[ P(A).main12() @ &m : res ] 
- = Pr[ W(T2).main() @ &m : res ].
-byequiv (_: ={glob A} ==> _). proc. inline*. sim. 
-rnd. skip. smt. auto. auto.
+lemma d_b2  (ii2 : at2)  &m : Pr[ P(A).main12(ii2) @ &m : res ] 
+  = f (Pr[ A.run1(ii2) @ &m : res ] - Pr[ A.run2(ii2) @ &m : res ]) .
+have ->: Pr[ P(A).main12(ii2) @ &m : res ]
+ = Pr[ W(T2).main(witness,ii2) @ &m : res ].
+byequiv (_: ={glob A} /\ arg{1} = arg.`2{2} ==> _). proc. inline*. 
+seq 1 3 : (={glob A} /\ b{1} = b{2} /\ i1i2.`2{2} = i2{1}).
+wp. 
+rnd. skip. smt. auto. 
+if. auto. call (_:true). skip. auto.
+wp. sim. call (_:true). skip. auto. auto. auto.
+
+
 rewrite (splitcases T2).
-have ->: Pr[T2.main(false, tt) @ &m : res] 
- = Pr[ A.run2() @ &m : !res ].
-byequiv. proc*. inline*. rcondf {1} 3. progress. wp. 
+have ->: Pr[T2.main(false, (witness,ii2)) @ &m : res]
+ = Pr[ A.run2(ii2) @ &m : !res ].
+byequiv. proc*. inline*. rcondf {1} 3. progress. wp.
 skip.  smt.
-wp.   sim. auto. auto.
-have ->: Pr[T2.main(true, tt) @ &m : res] 
- = Pr[ A.run1() @ &m : res ].
-byequiv. proc*. inline*. rcondt {1} 3. progress. wp. 
+wp.   sim.  
+call (_:true).  wp.  skip. progress. auto. auto.
+
+have ->: Pr[T2.main(true, (witness,ii2)) @ &m : res]
+ = Pr[ A.run1(ii2) @ &m : res ].
+byequiv. proc*. inline*. rcondt {1} 3. progress. wp.
 skip.  smt.
-wp.   sim. auto. auto.
-rewrite /f. 
-have -> : (1%r + (Pr[A.run1() @ &m : res] - Pr[A.run2() @ &m : res]))
- = Pr[A.run1() @ &m : res] + (1%r - Pr[A.run2() @ &m : res]).
+wp. call (_:true). wp. skip. auto. auto. auto.
+rewrite /f.
+have -> : (1%r + (Pr[A.run1(ii2) @ &m : res] - Pr[A.run2(ii2) @ &m : res]))
+ = Pr[A.run1(ii2) @ &m : res] + (1%r - Pr[A.run2(ii2) @ &m : res]).
 smt.
-have ->: (1%r - Pr[A.run2() @ &m : res]) = Pr[A.run2() @ &m : !res].
-   have -> : 1%r = Pr[A.run2() @ &m : true].
- byphoare.  conseq A_run2_ll.   auto. auto. 
+have ->: (1%r - Pr[A.run2(ii2) @ &m : res]) = Pr[A.run2(ii2) @ &m : !res].
+   have -> : 1%r = Pr[A.run2(ii2) @ &m : true].
+ byphoare.  conseq A_run2_ll.   auto. auto.
 rewrite Pr[mu_split res]. simplify. smt.
 smt.
 qed.
@@ -494,19 +512,19 @@ qed.
 
 
 
-lemma o_o &m p: 
-       p <=  Pr[ P(A).main1() @ &m : res ]  - 
-               Pr[ P(A).main2() @ &m : res ]
-   => exists &n, p <= Pr[ A.run1() @ &n : res ] - Pr[ A.run2() @ &n : res ].
+lemma o_o ii1 ii2 &m p: 
+       p <=  Pr[ P(A).main1(ii1,ii2) @ &m : res ]  - 
+               Pr[ P(A).main2(ii1,ii2) @ &m : res ]
+   => exists &n, p <= Pr[ A.run1(ii2) @ &n : res ] - Pr[ A.run2(ii2) @ &n : res ].
 progress.
-have f1 : Pr[P(A).main1() @ &m : res] - Pr[P(A).main2() @ &m : res]
-  = fop (Pr[ P(A).init_main12() @ &m : res ] ).
+have f1 : Pr[P(A).main1(ii1,ii2) @ &m : res] - Pr[P(A).main2(ii1,ii2) @ &m : res]
+  = fop (Pr[ P(A).init_main12(ii1,ii2) @ &m : res ] ).
 rewrite d_b1. smt.
-have f2 : p <= fop Pr[P(A).init_main12() @ &m : res].
+have f2 : p <= fop Pr[P(A).init_main12(ii1,ii2) @ &m : res].
 smt.
-have f3 : f p <= Pr[P(A).init_main12() @ &m : res]. smt.
-have f4 : exists &n,  f p <= Pr[ P(A).main12() @ &n : res ].
-apply (d_b3 &m (f p) (fun x => x)). auto.
+have f3 : f p <= Pr[P(A).init_main12(ii1,ii2) @ &m : res]. smt.
+have f4 : exists &n,  f p <= Pr[ P(A).main12(ii2) @ &n : res ].
+apply (d_b3  &m  (f p) (fun x => x) ii1 ii2). auto.
 elim f4. progress.
 exists &n.
 smt.
